ConcreteToSymbolicLemmas.v
@@ -105,7 +105,7 @@ Proof.
               eval_smt_arith (lookup_hdr s1 h) f).
   { unfold eval_sym_state.
     simpl.
-    rewrite commute_mapper_lookup_hdr.
+    rewrite commute_mapper_lookup_varlike.
     reflexivity. }
   rewrite H.
   destruct (Integers.eq (eval_smt_arith (lookup_hdr s1 h) f) v).
@@ -159,7 +159,7 @@ Lemma commute_sym_vs_conc_helper_seq_par_rule_hdr :
 Proof.
   intros mp hol f s1 h Hh.
   unfold eval_sym_state at 4.
-  rewrite commute_mapper_lookup_hdr.
+  rewrite commute_mapper_lookup_varlike.
   rewrite <- commute_state_hdr_updates.
   rewrite lookup_hdr_after_update_all_hdrs.
   -- destruct (eval_match_concrete mp (eval_sym_state s1 f)) eqn:Hmatch.
@@ -192,7 +192,7 @@ Lemma commute_sym_vs_conc_helper_seq_par_rule_sv :
 Proof.
   intros mp hol f s1 sv Hsv.
   unfold eval_sym_state at 4.
-  rewrite commute_mapper_lookup_state.
+  rewrite commute_mapper_lookup_varlike.
   rewrite lookup_state_after_update_all_states.
   -- destruct (eval_match_concrete mp (eval_sym_state s1 f)) eqn:Hmatch.
      + simpl.
