SmtQuery.v
@@ -116,8 +116,8 @@ Proof.
   rewrite commute_sym_vs_conc_transfomer_hdr.
   rewrite commute_sym_vs_conc_transfomer_hdr.
   unfold eval_sym_state.
-  rewrite commute_mapper_lookup_hdr.
-  rewrite commute_mapper_lookup_hdr.
+  rewrite commute_mapper_lookup_varlike.
+  rewrite commute_mapper_lookup_varlike.
   apply H_eq.
   assumption. assumption.
 Qed.
@@ -138,8 +138,8 @@ Proof.
   rewrite commute_sym_vs_conc_transfomer_sv.
   rewrite commute_sym_vs_conc_transfomer_sv.
   unfold eval_sym_state.
-  rewrite commute_mapper_lookup_state.
-  rewrite commute_mapper_lookup_state.
+  rewrite commute_mapper_lookup_varlike.
+  rewrite commute_mapper_lookup_varlike.
   apply H_eq.
   assumption. assumption.
 Qed.
@@ -160,8 +160,8 @@ Proof.
   rewrite commute_sym_vs_conc_transfomer_hdr.
   rewrite commute_sym_vs_conc_transfomer_hdr.
   unfold eval_sym_state.
-  rewrite commute_mapper_lookup_hdr.
-  rewrite commute_mapper_lookup_hdr.
+  rewrite commute_mapper_lookup_varlike.
+  rewrite commute_mapper_lookup_varlike.
   apply H.
   assumption. assumption.
 Qed.
@@ -182,8 +182,8 @@ Proof.
   rewrite commute_sym_vs_conc_transfomer_sv.
   rewrite commute_sym_vs_conc_transfomer_sv.
   unfold eval_sym_state.
-  rewrite commute_mapper_lookup_state.
-  rewrite commute_mapper_lookup_state.
+  rewrite commute_mapper_lookup_varlike.
+  rewrite commute_mapper_lookup_varlike.
   apply H.
   assumption. assumption.
 Qed.
